open import Relation.Binary using (StrictTotalOrder)

module BinaryTree.Elem
    {a ğ“â‚ ğ“â‚‚} (strictTotalOrder : StrictTotalOrder a ğ“â‚ ğ“â‚‚) where

open import Data.Empty using (âŠ¥)
open import Data.Nat using (â„•; suc; _+_)
open import Data.Nat.Properties using (+-suc; +-assoc)
open import Data.Product using (_Ã—_; _,_; projâ‚; projâ‚‚)
open import Data.Sum using (_âŠ_; injâ‚; injâ‚‚)
open import Level using (Level; _âŠ”_)
open import Relation.Binary using (_Respects_; Tri; tri<; triâ‰ˆ; tri>)
open import Relation.Binary.PropositionalEquality using (refl)
open import Relation.Nullary using (Â¬_; Dec; yes; no)
open import Relation.Nullary.Negation using (contradiction; contraposition)
open import Relation.Nullary.Sum using (_Â¬-âŠ_)
open StrictTotalOrder strictTotalOrder renaming (Carrier to A)

open import BinaryTree.Base (strictTotalOrder)

Â¬-Ã— : âˆ€ {p q : Level} {P : Set p} {Q : Set q} â†’ Â¬ P â†’ Â¬ (P Ã— Q)
Â¬-Ã— Â¬P = contraposition projâ‚ Â¬P

Ã—-Â¬ : âˆ€ {p q : Level} {P : Set p} {Q : Set q} â†’ Â¬ Q â†’ Â¬ (P Ã— Q)
Ã—-Â¬ Â¬Q = contraposition projâ‚‚ Â¬Q

infixr 6 _âˆˆ_

data _âˆˆ_ {l u : Aâº} : {h : â„•} â†’ A â†’ Tree l u h â†’ Set (a âŠ” ğ“â‚ âŠ” ğ“â‚‚) where
    here : âˆ€ {x y : A} {hË¡ hÊ³ : â„•} {nodeË¡ : Tree l [ y ] hË¡} {nodeÊ³ : Tree [ y ] u hÊ³}
         â†’ x â‰ˆ y
         â†’ x âˆˆ (node y nodeË¡ nodeÊ³)
    left : âˆ€ {x y : A} {hË¡ hÊ³ : â„•} {nodeË¡ : Tree l [ y ] hË¡} {nodeÊ³ : Tree [ y ] u hÊ³}
         â†’ l <âº [ x ]
         â†’ x < y
         â†’ x âˆˆ nodeË¡
         â†’ x âˆˆ (node y nodeË¡ nodeÊ³)
    right : âˆ€ {x y : A} {hË¡ hÊ³ : â„•} {nodeË¡ : Tree l [ y ] hË¡} {nodeÊ³ : Tree [ y ] u hÊ³}
          â†’ y < x
          â†’ [ x ] <âº u
          â†’ x âˆˆ nodeÊ³
          â†’ x âˆˆ (node y nodeË¡ nodeÊ³)

infixr 6 _âˆ‰_
_âˆ‰_ : âˆ€ {l u : Aâº} {h : â„•} â†’ A â†’ Tree l u h â†’ Set (a âŠ” ğ“â‚ âŠ” ğ“â‚‚)
x âˆ‰ tree = Â¬ (x âˆˆ tree)

xâˆˆtreeâ‡’xâˆˆnodeË¡âˆ¨xâˆˆnodeÊ³ : âˆ€ {l u : Aâº}
                           {x y : A}
                           {hË¡ hÊ³ : â„•}
                           {nodeË¡ : Tree l [ y ] hË¡}
                           {nodeÊ³ : Tree [ y ] u hÊ³}
                       â†’ x âˆˆ (node y nodeË¡ nodeÊ³)
                       â†’ x â‰ˆ y
                       âŠ (l <âº [ x ]) Ã— (x < y) Ã— (x âˆˆ nodeË¡)
                       âŠ (y < x) Ã— ([ x ] <âº u) Ã— (x âˆˆ nodeÊ³)
xâˆˆtreeâ‡’xâˆˆnodeË¡âˆ¨xâˆˆnodeÊ³ (here xâ‰ˆy) = injâ‚ xâ‰ˆy
xâˆˆtreeâ‡’xâˆˆnodeË¡âˆ¨xâˆˆnodeÊ³ (left l<x x<y xâˆˆnodeË¡) = injâ‚‚ (injâ‚ (l<x , (x<y , xâˆˆnodeË¡)))
xâˆˆtreeâ‡’xâˆˆnodeË¡âˆ¨xâˆˆnodeÊ³ (right y<x x<u xâˆˆnodeÊ³) = injâ‚‚ (injâ‚‚ (y<x , (x<u , xâˆˆnodeÊ³)))

elem? : âˆ€ {l u : Aâº} {h : â„•}
      â†’ (x : A)
      â†’ (tree : Tree l u h)
      â†’ l <âº [ x ]
      â†’ [ x ] <âº u
      â†’ Dec (x âˆˆ tree)
elem? x (leaf _) _ _ = no Î» ()
elem? x (node y _ _) _ _ with compare x y
elem? x (node y nodeË¡ nodeÊ³) l<x x<u | tri< x<y xâ‰‰y xâ‰¯y with elem? x nodeË¡ l<x [ x<y ]á´¿
... | yes xâˆˆnodeË¡ = yes (left l<x x<y xâˆˆnodeË¡)
... | no xâˆ‰nodeË¡ = let contra = xâ‰‰y Â¬-âŠ (Ã—-Â¬ (Ã—-Â¬ xâˆ‰nodeË¡)) Â¬-âŠ (Â¬-Ã— xâ‰¯y)
                   in no (contraposition xâˆˆtreeâ‡’xâˆˆnodeË¡âˆ¨xâˆˆnodeÊ³ contra)
elem? _ _ _ _ | triâ‰ˆ _ xâ‰ˆy _ = yes (here xâ‰ˆy)
elem? x (node y nodeË¡ nodeÊ³) l<x x<u | tri> xâ‰®y xâ‰‰y x>y with elem? x nodeÊ³ [ x>y ]á´¿ x<u
... | yes xâˆˆnodeÊ³ = yes (right x>y x<u xâˆˆnodeÊ³)
... | no xâˆ‰nodeÊ³ = let contra = xâ‰‰y Â¬-âŠ (Ã—-Â¬ (Â¬-Ã— xâ‰®y)) Â¬-âŠ (Ã—-Â¬ (Ã—-Â¬ xâˆ‰nodeÊ³))
                   in no (contraposition xâˆˆtreeâ‡’xâˆˆnodeË¡âˆ¨xâˆˆnodeÊ³ contra)

tree-x<u-âˆ§-l<xâ‡’tree-l<u : âˆ€ {l u : Aâº} {h : â„•} {x : A}
                        â†’ Tree [ x ] u h
                        â†’ l <âº [ x ]
                        â†’ Tree l u h
tree-x<u-âˆ§-l<xâ‡’tree-l<u (leaf x<u) l<x = leaf (transâº l<x x<u)
tree-x<u-âˆ§-l<xâ‡’tree-l<u (node x nodeË¡ nodeÊ³) l<x =
    node x (tree-x<u-âˆ§-l<xâ‡’tree-l<u nodeË¡ l<x) nodeÊ³

merge : âˆ€ {l u : Aâº} {hË¡ hÊ³ : â„•} {x : A}
      â†’ Tree l [ x ] hË¡
      â†’ Tree [ x ] u hÊ³
      â†’ Tree l u (hË¡ + hÊ³)
merge (leaf l<x) treeâ‚ = tree-x<u-âˆ§-l<xâ‡’tree-l<u treeâ‚ l<x
merge {hÊ³ = hÊ³} (node {hË¡ = hË¡Ë¡} {hÊ³ = hÊ³Ë¡} x nodeË¡ nodeÊ³) treeâ‚
    rewrite +-assoc hË¡Ë¡ hÊ³Ë¡ hÊ³ = node x nodeË¡ (merge nodeÊ³ treeâ‚)

delete : âˆ€ {l u : Aâº} {h : â„•} {x : A}
       â†’ (tree : Tree l u (suc h))
       â†’ x âˆˆ tree
       â†’ Tree l u h
delete (node _ nodeË¡ nodeÊ³) (here _) = merge nodeË¡ nodeÊ³
delete (node x nodeË¡@(node _ _ _) nodeÊ³) (left _ _ xâˆˆnodeË¡) =
    node x (delete nodeË¡ xâˆˆnodeË¡) nodeÊ³
delete (node {hË¡ = hË¡} x nodeË¡ nodeÊ³@(node {hË¡ = hË¡Ê³} {hÊ³ = hÊ³Ê³} _ _ _))
    (right _ _ xâˆˆnodeÊ³)
    rewrite +-suc hË¡ (hË¡Ê³ + hÊ³Ê³) = node x nodeË¡ (delete nodeÊ³ xâˆˆnodeÊ³)
